exercise-files/chap1-RHL.ec
@@ -2,8 +2,14 @@ pragma Goals: printall.
 
 require import AllCore.
 
+(*
+Let us work with Relational Hoare Logic and see how
+to handle it in EasyCryt. As usual let us start simple and
+define two functions that swap variables.
+*)
+
 module Jumbled = {
-  proc exchange1 (x y: int) : int*int = {
+  proc swap1 (x y: int) : int*int = {
   var z;
   z <- x;
   x <- y;
@@ -11,7 +17,7 @@ module Jumbled = {
   return (x,y);
   }
 
-  proc exchange2 (x y: int) : int*int = {
+  proc swap2 (x y: int) : int*int = {
   var z;
   z <- y;
   y <- x;
@@ -20,22 +26,135 @@ module Jumbled = {
   }
 }.
 
-lemma exchanges_equivalent: equiv [Jumbled.exchange1 ~  Jumbled.exchange2 : ={x, y} ==> ={res}  ].
+(*
+A couple of things to observe in the definitions.
+Firstly, they infact swap variables, however the order in which
+they swap them is different.
+Secondly, the return type of the functions is a tuple.
+Notice the syntax of how it is done. (int*int)
+
+On paper we define hoare quadruples like so:
+{P} C1 ~ C2 {Q}
+While in EC, we use the following syntax to say the same:
+equiv [C1 ~ C2 := P ==> Q]
+As with Hoare triples in EC, we access the results of both the programs using the
+"res" keyword. The numbers in the curly braces are the identifiers.
+So res{1} should be read as result from program 1.
+Let us first prove that swap1 is equivalent to itself.
+*)
+lemma swap1_equiv_swap1:
+equiv [Jumbled.swap1 ~  Jumbled.swap1 : x{1}=x{2} /\ y{1}=y{2} ==> res{1} = res{2}].
 proof.
 proc.
 simplify.
-wp 2 2.
-wp 1 1.
-wp.
+auto.
+qed.
+
+(*
+Let us now prove that both the swap functions are equivalent.
+Notice the shorthand that we use for the conditions.
+The eagle-eyed readers would've noticed this shorthand in the goals pane
+in the previous exercise.
+*)
+
+lemma swaps_equivalent:
+equiv [Jumbled.swap1 ~  Jumbled.swap2 : ={x, y} ==> ={res}  ].
+proof.
+proc.
+simplify.
+(*
+Now we have different programs, and the way we work with them is by using similar tactics
+that we used for HL. The only difference now is that we have to add identifiers 
+to the tactics for them to target specific sides and lines of code.
+For instance, for the sake of a demonstration let us use the wp tactic
+in an asymmetric way.
+*)
+wp 1 2.
+(*
+wp n1 n2: Consumes exactly n1 lines of the first program,
+and n2 lines of the second program.
+*)
+wp 0 1.
+wp 0 0.
+(* TODO: Strange behaviour (Inconsistent with the manual) *)
 skip.
 trivial.
 qed.
 
-(* Introduce the concept of adversary and games *)
+(*
+To be fair, the equivalence of swap1 and swap2
+is quite easy to prove, let us use the power of auto to
+clean up the proof.
+*)
+
+lemma swaps_equivalent_clean:
+equiv [Jumbled.swap1 ~  Jumbled.swap2 : ={x, y} ==> ={res}  ].
+proof.
+proc.
+auto.
+qed.
+
+(*
+Now let us take a small detour here and build on the the module types
+that we breifly introduced in the execise file of HL.
+When working with cryptography, we generally don't know about the
+inner workings of an adversary or an oracle.
+In order to model these in EC we have the module types.
+*)
+
 module type Adv = {
   proc eavesdrop_one(): bool
   proc eavesdrop_two(): bool
 }.
+
+(*
+By defining the module type Adv, we are instructing EC, that any
+concrete module which is of the Adv type has to, at the very least,
+implement eavesdrop_one, and eavesdrop_two procedures.
+What is interesting is that EC allows us to reason with the
+abstract module types as well. For example let us define a module
+which expects an Adv as input, and has a procedure called
+*)
+
+module Abstract_game(A:Adv) = {
+  proc one(): bool = {
+      var x;
+      x <- A.eavesdrop_one();
+      return x;
+  }
+}.
+
+(*
+At this stage, we don't know what A.eavesdrop_one does.
+Neither does EC. However, we can still prove certain facts
+related to it. Let us take a look at a simple example reflexivity
+example to understand how that works.
+Notice that we have a new term glob A, in the precondition.
+It stands for the global variable of the module A.
+So in this next lemma we claim that, if the global state of the A
+which is of type Adv is equal at the beginning of the program
+then running the same program yields us the same result.
+Quite a simple lemma, however the point to note here is
+that we haven't defined what the function is.
+*)
+
+lemma eavesdrop_reflex(A<:Adv):
+equiv [Abstract_game(A).one ~ Abstract_game(A).one : ={glob A} ==> ={res} ].
+proof.
+proc.
+call (_: true).
+(*
+TODO: How do I explain this?
+Manual is a bit messy as usual.
+*)
+auto.
+qed.
+
+(*
+However, let us also define a concrete instantiation of Adv,
+and reason with it. A is quite basic, and either always returns
+true or always returns false.
+*)
 
 module A : Adv = {
   proc eavesdrop_one() = {
@@ -59,12 +178,22 @@ inline *.
 wp.
 simplify.
 trivial.
+(* auto can replace wp. simplify. trivial  *)
 qed.
 
 (*
-As we discussed in the textbook, one of the use cases of RHL
-is to ensure that compiler optimizations do not modify program
-behaviour.
+The point of this detour is that,
+when we work with cryptographic proofs we will
+be dealing with adversaries both concrete and abstract ones,
+and we warming up and getting comfortable with EasyCrypt's
+tactics and ways.
+*)
+
+(*
+Before we move on to other things, let us take a look at
+something non-trivial in RHL.
+As we discussed earlier, one of the use cases of RHL
+is to ensure that compiler optimizations preserve program behaviour.
 Let us take a look at an example of this with a simple compiler
 optimization called invariant hoisting.
 Take a look at the programs defined below.
@@ -78,6 +207,13 @@ module Compiler = {
     }
     return (x,y);
   }
+
+  (*
+  As you can observe, the variable x is not affected by the loop,
+  hence to save computation, the compiler hoists that line out
+  of the scope of the while loop. Like so:
+  *)
+
   proc optimized (x y z: int) : int*int = {
     x <- z + 1;
     while (y < z){
@@ -87,12 +223,22 @@ module Compiler = {
   }
 }.
 
+(*
+Now let us try to prove the fact that
+the behaivour of both the programs is equivalent.
+*)
 lemma optimization_correct: equiv [Compiler.unoptimized ~  Compiler.optimized : ={x, y ,z} ==> ={res}  ].
 proof.
 proc.
 sp.
 simplify.
 
-  (* TODO: Help *)
+
+(* swap {1} (1.2) 1. *)
+(* TODO: Help *)
 
 while ( y{1} < z{1} /\ y{2} < z{2}).
+
+(*
+TODO: Non-trivial RHL exercises.
+*)
